Added examples from JAR paper to Containers and Collections

thys/Collections/Examples/Autoref/Simple_DFS.thy
@@ -5,149 +5,487 @@ imports
 begin
 
 
-text {*
-  This example presents the usage of the recursion combinator
-  @{text "RECT"}. The usage of the partial correct version 
-  @{text "REC"} is similar.
 
+section \<open>Graphs Implemented by Successor Function\<close>
+subsection \<open>Refinement relation\<close>
+definition "E_of_succ succ \<equiv> {(u,v). v\<in>succ u}"
+definition [to_relAPP]: "succg_rel R \<equiv> (R \<rightarrow> \<langle>R\<rangle>list_set_rel) O br E_of_succ (\<lambda>_. True)"
+
+
+consts i_graph :: "interface \<Rightarrow> interface"
+  \<comment> \<open>Define the conceptual type of graphs.\<close>
+
+lemmas [autoref_rel_intf] = REL_INTFI[of "succg_rel" i_graph]
+  \<comment> \<open>Declare \<open>succg_rel\<close> to be a relator for graphs.\<close>
+
+
+lemma in_id_succg_rel_iff: "(s,E)\<in>\<langle>Id\<rangle>succg_rel \<longleftrightarrow> (\<forall>v. distinct (s v) \<and> set (s v) = E``{v})"  
+  \<comment> \<open>Simplification in case of identity refinements for nodes\<close>
+  unfolding succg_rel_def br_def E_of_succ_def list_set_rel_def
+  by (auto; force dest: fun_relD)
+  
+  
+subsection \<open>Successor Operation\<close>
+definition [simp]: "op_succ E u \<equiv> E``{u}"
+  \<comment> \<open>Define the abstract successor operation.\<close>
+
+context begin interpretation autoref_syn .
+  lemma [autoref_op_pat]: "E``{v} \<equiv> op_succ$E$v" by simp
+  \<comment> \<open>Declare a rewrite rule to operation identification.\<close>
+end
+
+lemma refine_succg_succs[autoref_rules]: 
+  "(\<lambda>succs v. succs v,op_succ)\<in>\<langle>R\<rangle>succg_rel\<rightarrow>R\<rightarrow>\<langle>R\<rangle>list_set_rel"
+  \<comment> \<open>Declare implementation of successor function to Autoref.\<close>
+  apply (intro fun_relI)
+  apply (auto simp add: succg_rel_def br_def E_of_succ_def dest: fun_relD)
+  done
+
+section \<open>DFS Algorithm\<close>
+text {*
   We define a simple DFS-algorithm, prove a simple correctness
   property, and do data refinement to an efficient implementation.
 *}
 
 subsection {* Definition *}
-(* TODO: Warning, this is not exactly DFS, as V is not updated in FOREACH.
-  Replace by more accurate example from ICFContainers paper draft! *)
+
 text {* Recursive DFS-Algorithm. 
-  @{text "E"} is the edge relation of the graph, @{text "vd"} the node to 
-  search for, and @{text "v0"} the start node.
+  @{text "E"} is the edge relation of the graph, @{text "tgt"} the node to 
+  search for, and @{text "src"} the start node.
   Already explored nodes are 
   stored in @{text "V"}.*}
-definition dfs :: "('a \<Rightarrow>'a set) \<Rightarrow> 'a \<Rightarrow> 'a \<Rightarrow> bool nres" 
-  where
-  "dfs succ vd v0 \<equiv> REC\<^sub>T (\<lambda>D (V,v). 
-    if v=vd then RETURN True 
-    else if v\<in>V then RETURN False
-    else do {
-      let V=insert v V;
-      FOREACH\<^sub>C (succ v) ((=) False) (\<lambda>v' _. D (V,v')) False }
-  ) ({},v0)"
 
-subsection {* Correctness *}
+context 
+  fixes E :: "('v\<times>'v) set" and src :: 'v and tgt :: 'v
+begin
+  definition dfs :: "bool nres" where
+    "dfs \<equiv> do {
+      (_,r) \<leftarrow> RECT (\<lambda>dfs (V,v). 
+        if v=tgt then RETURN (V,True)
+        else do {
+          let V = insert v V;
+          FOREACHc (E``{v}) (\<lambda>(V,brk). \<not>brk) (\<lambda>v' (V,brk). 
+            if v'\<notin>V then dfs (V,v') else RETURN (V,False)
+          ) (V,False)
+        }) ({},src);
+      RETURN r
+    }"
 
-text {* As simple correctness property, we show:
-  If the algorithm returns true, then @{text "vd"} is reachable from 
-  @{text "v0"}.
-*}
-lemma dfs_sound:
-  fixes succ
-  defines "E \<equiv> {(v,v'). v'\<in>succ v}"
-  assumes F: "finite {v. (v0,v)\<in>E\<^sup>*}"
-  shows "dfs succ vd v0 \<le> SPEC (\<lambda>r. r \<longrightarrow> (v0,vd)\<in>E\<^sup>*)"
-proof -
-  have S: "\<And>v. succ v = E``{v}"
-    by (auto simp: E_def)
+  definition "reachable \<equiv> {v. (src,v)\<in>E\<^sup>*}"
+
+subsection \<open>Correctness Proof\<close>  
+  lemma dfs_correct:
+    assumes FIN: "finite (E\<^sup>*``{src})"
+    shows "dfs \<le> SPEC (\<lambda>r. r \<longleftrightarrow> (src,tgt)\<in>E\<^sup>*)"
+  proof -
+    from FIN have [simp, intro!]: "finite reachable"
+      unfolding reachable_def by (auto simp: Image_def)
+
+    text \<open>We first define the (inductive) pre and postconditions for 
+      the recursion, and the loop invariant\<close>  
+          
+    define rpre where "rpre \<equiv> \<lambda>S (V,v). 
+        v\<in>reachable - V 
+      \<and> V\<subseteq>reachable
+      \<and> S\<subseteq>V
+      \<and> tgt\<notin>V
+      \<and> E``(V-S) \<subseteq> V"
+
+    define rpost where "rpost \<equiv> \<lambda>S (V,v) (V',r). 
+          (r\<longrightarrow>tgt\<in>reachable) 
+        \<and> (\<not>r \<longrightarrow> 
+            tgt\<notin>V'
+          \<and> V\<subseteq>V' 
+          \<and> v\<in>V'
+          \<and> V'\<subseteq>reachable
+          \<and> E``(V'-S) \<subseteq> V'
+          )
+      "
+
+    define fe_inv where "fe_inv \<equiv> \<lambda>S V v it (V',r).
+        (r\<longrightarrow>tgt\<in>reachable)
+      \<and> (\<not>r \<longrightarrow> 
+          tgt \<notin> V'
+        \<and> insert v V\<subseteq>V'
+        \<and> E``{v} - it \<subseteq> V'
+        \<and> V'\<subseteq>reachable
+        \<and> S\<subseteq>insert v V
+        \<and> E``(V'-S) \<subseteq> V' \<union> it 
+        \<and> E``(V'-insert v S) \<subseteq> V'
+        )"
+
+    text \<open>Then we prove the verification conditions that our VCG will generate as separate facts.
+      Of course, the workflow is to first let run the VCG, and then extract these facts from 
+      its output. This way, we can make explicit the ideas of the proof, and present them separately 
+      from the mainly technical VC generation.
+     \<close>
+        
+    have vc_pre_initial: "rpre {} ({}, src)"
+      by (auto simp: rpre_def reachable_def)
+
+    {
+      (* Case: Found node *)
+      fix S V
+      assume "rpre S (V,tgt)"
+      hence "rpost S (V,tgt) (insert tgt V, True)"
+        unfolding rpre_def rpost_def
+        by auto
+    } note vc_node_found = this
+
+    { (* The set of nodes that the foreach loop iterates over is finite *)
+      fix S V v
+      assume "rpre S (V, v)"
+      hence "finite (E``{v})"
+        unfolding rpre_def reachable_def
+        using FIN  
+        apply auto
+        by (meson finite_Image_subset finite_reachable_advance r_le_rtrancl)
+    } note vc_foreach_finite = this
   
-  from F show ?thesis
-    unfolding dfs_def S
-    apply (refine_rcg refine_vcg impI
-      RECT_rule[where 
-        pre="\<lambda>(V,v). (v0,v)\<in>E\<^sup>* \<and> V\<subseteq>{v. (v0,v)\<in>E\<^sup>*}" and
-        V="finite_psupset ({v. (v0,v)\<in>E\<^sup>*}) <*lex*> {}"]
-      FOREACHc_rule[where I="\<lambda>_ r. r \<longrightarrow> (v0, vd) \<in> E\<^sup>*"]
-    )
+    {
+      (* fe_inv initial *)
+      fix S V v
+      assume A: "v \<notin> V" "v \<noteq> tgt"
+        and PRE: "rpre S (V, v)"
+      hence "fe_inv S V v (E``{v}) (insert v V, False)"
+        unfolding fe_inv_def rpre_def by (auto simp: )
+    } note vc_enter_foreach = this
 
-    apply (auto intro: finite_subset[of _ "{v'. (v0,v')\<in>E\<^sup>*}"])
-    apply rprems
-    apply (auto simp: finite_psupset_def)
-    done    
-qed
+    {
+      (* fe_inv ensures rpre *)
+      fix S V v v' it V'
+      assume A: "v'\<notin>V'" "v' \<in> it" "it \<subseteq> E``{v}"
+        and FEI: "fe_inv S V v it (V', False)"
+        and PRE: "rpre S (V, v)"
+
+      from A have "(v,v')\<in>E" by auto
+      moreover from PRE have "v \<in> reachable" by (auto simp: rpre_def)
+      hence "E``{v} \<subseteq> reachable" by (auto simp: reachable_def)
+      ultimately have [simp]: "v'\<in>reachable" by blast
+
+      from A FEI PRE have "rpre (insert v S) (V', v')"
+        unfolding rpre_def fe_inv_def by auto
+    } note vc_rec_pre = this
+
+    {
+      (* rpost implies fe_inv *)
+      fix S V V' v v' it Vr''
+      assume "fe_inv S V v it (V', False)"
+        and "rpost (insert v S) (V', v') Vr''"
+      hence "fe_inv S V v (it - {v'}) Vr''"
+        unfolding rpre_def rpost_def fe_inv_def by clarsimp (auto; blast)
+    } note vc_iterate_foreach = this
+
+    { (* Recursive call in variant relation *)
+      fix S V V' v it
+      assume "rpre S (V, v)"  
+      and "fe_inv S V v it (V', False)"
+      hence "(V',V)\<in>finite_psupset local.reachable"
+        unfolding fe_inv_def rpre_def
+        by (auto simp: finite_psupset_def)
+      
+    } note vc_rec_var = this
+      
+    {
+      (* fe_inv preserved if ignoring visitied node*)
+      fix S V V' v v' it Vr''
+      assume "fe_inv S V v it (V', False)"
+        and "v'\<in>V'"
+      hence "fe_inv S V v (it - {v'}) (V', False)"
+        unfolding fe_inv_def by auto
+    } note vc_foreach_ignore = this
+
+
+    {
+      (* fe_inv (completed) implies rpost *)
+      fix S V v V'
+      assume FEI: "fe_inv S V v {} (V', False)"
+      have "rpost S (V, v) (V', False)"
+        unfolding rpost_def
+        using FEI by (auto simp: fe_inv_def) []
+    } note vc_foreach_completed_imp_post = this
+
+    {
+      (* fe_inv (interrupted) implies rpost *)
+      fix S V v V' it
+      assume FEI: "fe_inv S V v it (V', True)"
+      hence "rpost S (V, v) (V', True)"
+        by (auto simp add: rpost_def fe_inv_def) []
+    } note vc_foreach_interrupted_imp_post = this
+
+    { (* The postcondition of the recursion implies our desired specification *)
+      fix V r
+      assume "rpost {} ({}, src) (V, r)"
+      hence "r = ((src, tgt) \<in> E\<^sup>*)"
+        by (auto 
+          simp: rpost_def reachable_def 
+          dest: Image_closed_trancl 
+          intro: rev_ImageI)
+    } note vc_rpost_imp_spec = this
+
+    text \<open>The verification condition generation is technical. We invoke the VCG,
+      and discharge the generated VCs. The trivial ones are discharged on the spot, the
+      more complicated ones have been extracted to separate facts, that we use in the proof 
+      text below.
+    \<close>
+    show ?thesis
+      unfolding dfs_def
+      apply (refine_vcg RECT_rule_arb[
+        where 
+              pre=rpre and arb="{}"
+          and M="\<lambda>a x. SPEC (rpost a x)"
+          and V="inv_image (finite_psupset reachable) fst", 
+        THEN order_trans
+        ])
+      subgoal by blast  (* Well-Foundedness  *)
+      subgoal by (rule vc_pre_initial)
+      subgoal by (auto simp add: rpre_def rpost_def) (* Found tgt node *)
+      
+      subgoal for f S _ V v (* Entering inner FOREACH loop *)
+        apply (refine_rcg refine_vcg 
+          FOREACHc_rule'[where I="fe_inv S V v" (*for S V*)]
+          )
+        apply clarsimp_all
+
+        subgoal by (simp add: vc_foreach_finite) (* Finiteness of iteration set *)
+
+        subgoal by (rule vc_enter_foreach) (simp add: rpre_def) (* Loop invar holds initially*)
+        subgoal (* Loop invar preserved by inner recursion *)
+          apply (rule order_trans, rprems)   (* Applying recursion induction hypothesis *)
+          apply (erule (4) vc_rec_pre; fail) (* Precondition of inner recursion holds*)
+          apply (simp add: vc_rec_var; fail) (* Parameters are smaller wrt termination ordering *)
+          apply (auto simp: vc_iterate_foreach; fail) (* Postcondition of inner rec implies loop invar again  *)
+          done
+          
+        subgoal by (rule vc_foreach_ignore; auto)  (* Node already visited: invariant is preserved *)
+        subgoal by (auto simp: vc_foreach_completed_imp_post) (* Foreach loop terminated normally: Implies postcondition *)
+        subgoal by (auto simp: vc_foreach_interrupted_imp_post) (* Foreach loop interrupted (tgt found): Implies postcondition *)
+        done
+      subgoal by (auto simp add: vc_rpost_imp_spec) (* Postcondition implies our specification *)
+      done
+    qed
+    
+end
+
 
 subsection {* Data Refinement and Determinization *}
+
 text {*
   Next, we use automatic data refinement and transfer to generate an
-  executable algorithm. The edges function
-  is refined to a successor function returning a list-set.
+  executable algorithm. We fix the node-type to natural numbers,
+  and the successor-function to return a list-set. 
+  The implementation of the visited set is left open, and Autoref's heuristics
+  will choose one (default for nat set: red-black-trees).
 *}
+
+text \<open>In our first example, we use \<open>autoref_monadic\<close>, which combines the 
+  Autoref tool and the determinization of the Monadic Refinement Framework.\<close>
+  
 schematic_goal dfs_impl_refine_aux:
-  fixes succi and succ :: "nat \<Rightarrow> nat set" and vd v0 :: nat
-  assumes [autoref_rules]: "(succi,succ)\<in>Id\<rightarrow>\<langle>Id\<rangle>list_set_rel"
-  notes [autoref_rules] = IdI[of v0] IdI[of vd]
-  shows "(?f::?'c, dfs succ vd v0)\<in>?R"
-  unfolding dfs_def[abs_def]
-  apply (autoref_monadic)
+  fixes succi and E :: "('a::linorder \<times> 'a) set" and tgt src :: 'a
+  assumes [autoref_rules]: "(succi,E)\<in>\<langle>Id\<rangle>succg_rel"
+  notes [autoref_rules] = IdI[of src] IdI[of tgt]
+  shows "RETURN (?f::?'c) \<le> \<Down>?R (dfs E src tgt)"
+  unfolding dfs_def by autoref_monadic 
+
+text \<open>We define a new constant from the synthesis result\<close>
+concrete_definition dfs_impl for succi src tgt uses dfs_impl_refine_aux
+text \<open>Set up code equations for the recursion combinators\<close>
+prepare_code_thms dfs_impl_def
+text \<open>And export the algorithm to all supported target languages\<close>
+export_code dfs_impl checking SML OCaml? Haskell? Scala
+
+
+text {* Chaining the refinement theorems, we get correctness arguments that 
+  are almost independent of the refinement framework: *}
+
+lemma succ_ran_fin:
+  assumes R: "(succi,E) \<in> \<langle>Rv\<rangle>succg_rel"
+  assumes "v\<in>Range Rv"
+  shows "finite (E``{v})"
+  using assms
+  unfolding succg_rel_def br_def E_of_succ_def
+  apply clarsimp
+  apply (drule (1) fun_relD)
+  using list_set_rel_range[of Rv]
+  by auto
+
+lemma run_ran_aux:
+  assumes R: "(succi,E) \<in> \<langle>Rv\<rangle>succg_rel"
+  assumes REACH: "(src,v)\<in>E\<^sup>*"
+  assumes R0: "(v0i,src) \<in> Rv"
+  shows "v \<in> Range Rv"
+  using REACH R0
+proof (induction arbitrary: v0i rule: converse_rtrancl_induct)
+  case base thus ?case by auto
+next
+  case (step src v')  
+  from \<open>(src, v') \<in> E\<close> have "v' \<in> Range Rv" using R list_set_rel_range[of Rv]
+    apply (clarsimp simp: succg_rel_def br_def E_of_succ_def)
+    apply (drule fun_relD[OF _ \<open>(v0i, src) \<in> Rv\<close>])
+    by auto
+  with step.IH show ?thesis by blast
+qed
+
+lemma run_ran_fin: 
+  assumes R: "(succi,E) \<in> \<langle>Rv\<rangle>succg_rel"
+  assumes R0: "(v0i,src) \<in> Rv"
+  shows "\<forall>v. (src,v)\<in>E\<^sup>* \<longrightarrow> finite (E``{v})"
+  using succ_ran_fin run_ran_aux assms by metis
+
+text \<open>Correctness theorem presented in the paper:\<close>
+theorem dfs_code_correct: 
+  assumes SUCCI: "(succi,E)\<in>\<langle>Id\<rangle>succg_rel"
+  assumes FIN: "finite (E\<^sup>*``{src})"  
+  shows "dfs_impl succi src tgt \<longleftrightarrow> (src,tgt)\<in>E\<^sup>*"
+proof -
+  note dfs_impl.refine[OF SUCCI, of src tgt]
+  also note dfs_correct[OF FIN]
+  finally show ?thesis by (auto simp: split: dres.split)
+qed
+
+subsubsection \<open>Using only Autoref\<close>
+
+text \<open>Here we show the result of Autoref, without the determinization phase of
+  the Monadic Refinement Framework: \<close>
+schematic_goal 
+  fixes succi and E :: "('a::linorder \<times> 'a) set" and tgt src :: 'a
+  assumes [autoref_rules]: "(succi,E)\<in>\<langle>Id\<rangle>succg_rel"
+  notes [autoref_rules] = IdI[of src] IdI[of tgt]
+  shows "(?f::?'c, dfs E src tgt) \<in> ?R"
+  unfolding dfs_def[abs_def] 
+  apply (autoref (trace))
   done
 
-text {* We can configure our tool to use different implementations.
-  Here, we use lists for sets of natural numbers. *}
+subsubsection \<open>Choosing Different Implementations\<close>
+text \<open>Ad-hoc override of implementation selection heuristics: Using hashset for the visited set\<close>  
 schematic_goal dfs_impl_refine_aux2:
-  fixes succi and succ :: "nat \<Rightarrow> nat set" and vd v0 :: nat
-  assumes [autoref_rules]: "(succi,succ)\<in>Id\<rightarrow>\<langle>Id\<rangle>dflt_rs_rel" 
-  notes [autoref_rules] = IdI[of v0] IdI[of vd]
-  notes [autoref_tyrel] = ty_REL[where 'a="nat set" and R="\<langle>Id\<rangle>list_set_rel"]
-  shows "(?f::?'c, dfs succ vd v0)\<in>?R"
-  unfolding dfs_def[abs_def]
-  apply (autoref_monadic)
+  fixes succi and E :: "(('a::hashable) \<times> 'a) set" and tgt src :: 'a
+  assumes [autoref_rules]: "(succi,E)\<in>\<langle>Id\<rangle>succg_rel"
+  notes [autoref_rules] = IdI[of src] IdI[of tgt]
+  notes [autoref_tyrel] = ty_REL[where 'a="'a set" and R="\<langle>Id\<rangle>dflt_ahs_rel"] 
+  shows "(?f::?'c, dfs E src tgt) \<in> ?R"
+  unfolding dfs_def[abs_def] 
+  apply autoref_monadic
   done
+  
 
 text {* We can also leave the type of the nodes and its implementation
-  unspecified. However, the implementation relation must be single-valued,
-  and we need a comparison operator on nodes *}
-
-(*schematic_lemma 
-  fixes vs vd :: 'a and Rv :: "('c\<times>'a) set"
-  assumes [autoref_rules]: "(vsi,vs)\<in>Rv" "(vdi,vd)\<in>Rv" 
-  shows "(?f::?'c, vs = vd)\<in>?R"
-  apply (autoref (keep_goal) phases: id_op rel_inf fix_rel)
-*)
-
-
+  unspecified. However, we need a comparison operator on nodes *}
+  
+(* With linorder typeclass on abstract type *)  
 schematic_goal dfs_impl_refine_aux3:
-  fixes succi and succ :: "'a::linorder \<Rightarrow> 'a set" 
+  fixes succi and E :: "('a::linorder \<times> 'a) set" 
     and Rv :: "('ai\<times>'a) set"
   assumes [autoref_rules_raw]: "(cmpk, dflt_cmp (\<le>) (<))\<in>(Rv\<rightarrow>Rv\<rightarrow>Id)"
   notes [autoref_tyrel] = ty_REL[where 'a="'a set" and R="\<langle>Rv\<rangle>dflt_rs_rel"]
   assumes P_REF[autoref_rules]: 
-    "(succi,succ)\<in>Rv\<rightarrow>\<langle>Rv\<rangle>list_set_rel"
-    "(vdi,vd::'a)\<in>Rv"
-    "(v0i,v0)\<in>Rv"
-  shows "(?f::?'c, dfs succ vd v0)\<in>?R"
+    "(succi,E)\<in>\<langle>Rv\<rangle>succg_rel"
+    "(vdi,tgt::'a)\<in>Rv"
+    "(v0i,src)\<in>Rv"
+  shows "(RETURN (?f::?'c), dfs E src tgt)\<in>?R"
   unfolding dfs_def[abs_def]
   by autoref_monadic
 
-text {* Next, we extract constants from the refinement lemmas,
-  and prepare them for code-generation *}
-concrete_definition dfs_impl for succi vd ?v0.0 uses dfs_impl_refine_aux
-prepare_code_thms dfs_impl_def
-concrete_definition dfs_impl2 for succi vd ?v0.0 uses dfs_impl_refine_aux2
+(* With arbitrary cmpk' operator on abstract type, not forcing a linorder typeclass instance.
+  Useful if there are multiple possible instantiations of a typeclass (eg for product ordering), 
+  and one does not want to commit to one.
+*)  
+schematic_goal dfs_impl_refine_aux3':
+  fixes succi and E :: "('a \<times> 'a) set" 
+    and Rv :: "('ai\<times>'a) set"
+  assumes [autoref_ga_rules]: "eq_linorder cmpk'"
+  assumes [autoref_rules_raw]: "(cmpk, cmpk')\<in>(Rv\<rightarrow>Rv\<rightarrow>comp_res_rel)"
+  notes [autoref_tyrel] = ty_REL[where 'a="'a set" and R="\<langle>Rv\<rangle>map2set_rel (rbt_map_rel (comp2lt cmpk'))"]
+  assumes P_REF[autoref_rules]: 
+    "(succi,E)\<in>\<langle>Rv\<rangle>succg_rel"
+    "(vdi,tgt::'a)\<in>Rv"
+    "(v0i,src)\<in>Rv"
+  shows "(RETURN (?f::?'c), dfs E src tgt)\<in>?R"
+  unfolding dfs_def[abs_def]
+  by autoref_monadic
+  
+  
+text {* We also generate code for the alternative implementations *}
+concrete_definition dfs_impl2 for succi src tgt uses dfs_impl_refine_aux2
+concrete_definition dfs_impl3 for cmpk succi v0i vdi uses dfs_impl_refine_aux3
+concrete_definition dfs_impl3' for cmpk succi v0i vdi uses dfs_impl_refine_aux3'
+
 prepare_code_thms dfs_impl2_def
-concrete_definition dfs_impl3 for succi vd ?v0.0 uses dfs_impl_refine_aux3
 prepare_code_thms dfs_impl3_def
+prepare_code_thms dfs_impl3'_def
 
-text {* Finally, we export code using the code-generator *}
-export_code dfs_impl dfs_impl2 dfs_impl3 in SML
-export_code dfs_impl dfs_impl2 dfs_impl3 in OCaml
-export_code dfs_impl dfs_impl2 dfs_impl3 in Haskell
-export_code dfs_impl dfs_impl2 dfs_impl3 in Scala
+export_code dfs_impl dfs_impl2 dfs_impl3 dfs_impl3' checking SML OCaml? Haskell? Scala
 
-text {* Derived correctness lemma for the generated function *}
-lemma dfs_impl_correct:
-  fixes succi succ
-  defines "E \<equiv> {(s, s'). s' \<in> succ s}"
-  assumes S: "(succi,succ) \<in> Id \<rightarrow> \<langle>Id\<rangle>list_set_rel"
-  assumes F: "finite (E\<^sup>*``{v0})"
-  assumes R: "dfs_impl succi vd v0"
-  shows "(v0,vd)\<in>E\<^sup>*"
+text \<open>And we prove the alternative implementations correct \<close>
+
+theorem dfs_code2_correct: 
+  assumes SUCCI: "(succi,E)\<in>\<langle>Id\<rangle>succg_rel"
+  assumes FIN: "finite (E\<^sup>*``{src})"  
+  shows "dfs_impl2 succi src tgt \<longleftrightarrow> (src,tgt)\<in>E\<^sup>*"
 proof -
-  note dfs_impl.refine[OF S, of vd v0, THEN nres_relD]
-  also
-  have F': "finite {v. (v0, v) \<in> {(v, v'). v' \<in> succ v}\<^sup>*}" 
-    using F 
-    apply (fo_rule back_subst, assumption)
-    by (auto simp: E_def)
-  note dfs_sound[OF F']
-  finally show ?thesis using R 
-    by (auto simp: E_def)
-
+  note dfs_impl2.refine[OF SUCCI, of src tgt, THEN nres_relD]
+  also note dfs_correct[OF FIN]
+  finally show ?thesis by (auto simp: split: dres.split)
 qed
+  
+theorem dfs_code3_correct: 
+  fixes succi and succ :: "'a::linorder \<Rightarrow> 'a set" 
+    and Rv :: "('ai\<times>'a) set"
+  assumes V0: "(v0i,src)\<in>Rv"
+  assumes VD: "(vdi,tgt)\<in>Rv"
+  assumes SUCCI: "(succi,E)\<in>\<langle>Rv\<rangle>succg_rel"
+  assumes CMP: "(cmpk, dflt_cmp (\<le>) (<))\<in>(Rv\<rightarrow>Rv\<rightarrow>Id)"
+  assumes FIN: "finite (E\<^sup>*``{src})"  
+  shows "dfs_impl3 cmpk succi v0i vdi \<longleftrightarrow> (src,tgt)\<in>E\<^sup>*"
+proof -
+  note dfs_impl3.refine[OF CMP SUCCI VD V0, THEN nres_relD]
+  also note dfs_correct[OF FIN]
+  finally show ?thesis by (auto simp: split: dres.split)
+qed
+
+theorem dfs_code3'_correct: 
+  fixes succi and succ :: "'a::linorder \<Rightarrow> 'a set" 
+    and Rv :: "('ai\<times>'a) set"
+  assumes V0: "(v0i,src)\<in>Rv"
+  assumes VD: "(vdi,tgt)\<in>Rv"
+  assumes SUCCI: "(succi,E)\<in>\<langle>Rv\<rangle>succg_rel"
+  assumes CGA: "eq_linorder cmpk'"
+  assumes CMP: "(cmpk, cmpk') \<in> Rv\<rightarrow>Rv\<rightarrow>comp_res_rel"
+  assumes FIN: "finite (E\<^sup>*``{src})"  
+  shows "dfs_impl3' cmpk succi v0i vdi \<longleftrightarrow> (src,tgt)\<in>E\<^sup>*"
+proof -
+  note dfs_impl3'.refine[OF CGA CMP SUCCI VD V0, THEN nres_relD]
+  also note dfs_correct[OF FIN]
+  finally show ?thesis by (auto simp: split: dres.split)
+qed
+
+
+(* Reachability *)  
+
+definition [simp]: "op_reachable E u v \<equiv> (u,v)\<in>E\<^sup>*"
+context begin interpretation autoref_syn .
+  lemma [autoref_op_pat]: "(u,v)\<in>E\<^sup>* \<equiv> op_reachable$E$u$v" by simp
+
+
+  (* We use a quite general setup here, working with any linearly ordered
+    abstract node type, refined by any relation. *)
+  theorem dfs_code3_correct_rl[autoref_rules]: 
+    fixes succi and succ :: "'a::linorder \<Rightarrow> 'a set" 
+      and Rv :: "('ai\<times>'a) set"
+    assumes V0: "(v0i,src)\<in>Rv"
+    assumes VD: "(vdi,tgt)\<in>Rv"
+    assumes SUCCI: "(succi,E)\<in>\<langle>Rv\<rangle>succg_rel"
+    assumes CGA: "SIDE_GEN_ALGO (eq_linorder cmpk')"
+    assumes CMP: "GEN_OP cmpk cmpk' (Rv\<rightarrow>Rv\<rightarrow>comp_res_rel)"
+    assumes FIN: "SIDE_PRECOND (finite (E\<^sup>*``{src}))"  
+    shows "(dfs_impl3' cmpk succi v0i vdi, 
+          (OP op_reachable ::: \<langle>Rv\<rangle>succg_rel \<rightarrow> Rv \<rightarrow> Rv \<rightarrow> bool_rel)$E$src$tgt)
+          \<in> bool_rel"
+    using dfs_code3'_correct[OF V0 VD SUCCI, of cmpk' cmpk] CGA CMP FIN
+    unfolding autoref_tag_defs by simp
+    
+end
+
 
 end
