thys/Collections/Examples/Autoref/Collection_Autoref_Examples.thy
@@ -6,6 +6,7 @@ imports
   ICF_Test 
   ICF_Only_Test 
   Nested_DFS 
+  Combined_TwoSat
 begin
 end
 (*>*)
