thys/Collections/Refine_Dflt.thy
@@ -8,16 +8,30 @@ begin
 
 text {* Configurations *}
 
-lemmas tyrel_dflt_nat_set[autoref_tyrel] = 
+lemmas tyrel_dflt_nat_set = 
   ty_REL[where 'a="nat set" and R="\<langle>Id\<rangle>dflt_rs_rel"]
 
-lemmas tyrel_dflt_bool_set[autoref_tyrel] = 
+lemmas tyrel_dflt_bool_set = 
   ty_REL[where 'a="bool set" and R="\<langle>Id\<rangle>list_set_rel"]
 
-lemmas tyrel_dflt_nat_map[autoref_tyrel] = 
+lemmas tyrel_dflt_nat_map = 
   ty_REL[where R="\<langle>nat_rel,Rv\<rangle>dflt_rm_rel"] for R
 
-lemmas tyrel_dflt = tyrel_dflt_nat_set tyrel_dflt_bool_set tyrel_dflt_nat_map
+lemmas tyrel_dflt_old = tyrel_dflt_nat_set tyrel_dflt_bool_set tyrel_dflt_nat_map
+
+lemmas tyrel_dflt_linorder_set = 
+  ty_REL[where R="\<langle>Id::('a::linorder\<times>'a) set\<rangle>dflt_rs_rel"]
+  
+lemmas tyrel_dflt_linorder_map = 
+  ty_REL[where R="\<langle>Id::('a::linorder\<times>'a) set,R\<rangle>dflt_rm_rel"] for R
+  
+lemmas tyrel_dflt_bool_map = 
+  ty_REL[where R="\<langle>Id::(bool\<times>bool) set,R\<rangle>list_map_rel"] for R
+
+lemmas tyrel_dflt = tyrel_dflt_linorder_set tyrel_dflt_bool_set tyrel_dflt_linorder_map tyrel_dflt_bool_map
+
+declare tyrel_dflt[autoref_tyrel]
+
 
 
 local_setup {*
@@ -39,5 +53,29 @@ local_setup {*
     declare_prio "Gen-List-Map" @{term "\<langle>R\<rangle>list_map_rel"} PR_LAST
   end
 *}
+
+text \<open>Quick test of setup:\<close>
+context begin
+private schematic_goal test_dflt_tyrel1: "(?c::?'c,{1,2,3::int})\<in>?R" (*RBT*)
+  by autoref
+private lemmas asm_rl[of "_\<in>\<langle>int_rel\<rangle>dflt_rs_rel", OF test_dflt_tyrel1]
+
+private schematic_goal test_dflt_tyrel2: "(?c::?'c,{True, False})\<in>?R" (*List*)
+  by autoref
+private lemmas asm_rl[of "_\<in>\<langle>bool_rel\<rangle>list_set_rel", OF test_dflt_tyrel2]
+
+private schematic_goal test_dflt_tyrel3: "(?c::?'c,[1::int\<mapsto>0::nat])\<in>?R" (*RBT*)
+  by autoref
+private lemmas asm_rl[of "_\<in>\<langle>int_rel,nat_rel\<rangle>dflt_rm_rel", OF test_dflt_tyrel3]
+
+private schematic_goal test_dflt_tyrel4: "(?c::?'c,[False\<mapsto>0::nat])\<in>?R" (*List*)
+  by autoref
+private lemmas asm_rl[of "_\<in>\<langle>bool_rel,nat_rel\<rangle>list_map_rel", OF test_dflt_tyrel4]
+
+end
+
+
+
+
 
 end
